Add Begin/Commit to API
Need the code to indicate where transaction boundaries are somehow

src/dafny_go/jrnl/jrnl.go
@@ -1,7 +1,30 @@
 package jrnl
 
-import "github.com/mit-pdos/goose-nfsd/txn"
+import (
+	"github.com/mit-pdos/goose-nfsd/buftxn"
+	"github.com/mit-pdos/goose-nfsd/txn"
+	"github.com/tchajed/goose/machine/disk"
+)
+
+type Disk = disk.Disk
+type Txn struct {
+	btxn *buftxn.BufTxn
+}
 
 type Jrnl struct {
 	txn *txn.Txn
+}
+
+func NewJrnl(d Disk) *Jrnl {
+	return &Jrnl{txn: txn.MkTxn(d)}
+}
+
+func (jrnl *Jrnl) Begin() Txn {
+	return Txn{btxn: buftxn.Begin(jrnl.txn)}
+}
+
+// TODO: wrap read/write
+
+func (txn Txn) Commit() {
+	txn.btxn.CommitWait(true)
 }
