src/dafny_go/go.mod
@@ -5,4 +5,5 @@ go 1.15
 require (
 	github.com/mit-pdos/goose-nfsd v0.0.0-20201221203728-170cafdcddd9
 	github.com/stretchr/testify v1.6.1
+	github.com/tchajed/goose v0.0.0-20201215222528-5fb81fabc18d
 )
